new specs for hashing

specs/Spec.Hash.fst
@@ -1,28 +1,63 @@
 module Spec.Hash
 
+module S = FStar.Seq
 
-inline_for_extraction
-private let alg (a:algorithm) =
+open Spec.Hash.Definitions
+open Spec.Hash.PadFinish
+
+let init a: init_t a =
   match a with
-  | SHA2_224 -> Spec.SHA2.SHA2_224
-  | SHA2_256 -> Spec.SHA2.SHA2_256
-  | SHA2_384 -> Spec.SHA2.SHA2_384
-  | SHA2_512 -> Spec.SHA2.SHA2_512
+  | SHA2_224 | SHA2_256 | SHA2_384 | SHA2_512 ->
+      Spec.SHA2.init a
+  | MD5 ->
+      Spec.MD5.init
+  | SHA1 ->
+      Spec.SHA1.init
 
-let state (a:algorithm) =
+let update a: update_t a =
   match a with
-  | SHA2_224 -> Spec.SHA2.hash_w Spec.SHA2.SHA2_224
-  | SHA2_256 -> Spec.SHA2.hash_w Spec.SHA2.SHA2_256
-  | SHA2_384 -> Spec.SHA2.hash_w Spec.SHA2.SHA2_384
-  | SHA2_512 -> Spec.SHA2.hash_w Spec.SHA2.SHA2_512
+  | SHA2_224 | SHA2_256 | SHA2_384 | SHA2_512 ->
+      Spec.SHA2.update a
+  | MD5 ->
+      Spec.MD5.update
+  | SHA1 ->
+      Spec.SHA1.update
 
+(* A helper that deals with the modulo proof obligation to make things go smoothly. *)
+let split_block (a: hash_alg)
+  (blocks: bytes_blocks a)
+  (n: nat{n <= S.length blocks / block_length a}):
+  Tot (p:(Spec.Hash.Definitions.bytes_blocks a * Spec.Hash.Definitions.bytes_blocks a)
+         {fst p == fst (Seq.split blocks (FStar.Mul.(n * block_length a))) /\
+	  snd p == snd (Seq.split blocks (FStar.Mul.(n * block_length a)))})
+=
+  let block, rem = S.split blocks FStar.Mul.(n * block_length a) in
+  assert (S.length rem = S.length blocks - S.length block);
+  Math.Lemmas.modulo_distributivity (S.length rem) (S.length block) (block_length a);
+  assert (S.length rem % block_length a = 0);
+  block, rem
 
-let init (a:algorithm) = Spec.SHA2.init (alg a)
+(* Compression function for multiple blocks. Note: this one could be
+ * parameterized over any update function and the lemma would still be provable,
+ * but that's perhaps too much hassle. *)
+let rec update_multi
+  (a:hash_alg)
+  (hash:words_state a)
+  (blocks:bytes_blocks a):
+  Tot (words_state a) (decreases (S.length blocks))
+=
+  if S.length blocks = 0 then
+    hash
+  else
+    let block, rem = split_block a blocks 1 in
+    let hash = update a hash block in
+    update_multi a hash rem
 
-let update_block (a:algorithm) block chash = Spec.SHA2.update_block (alg a) block chash
+#reset-options "--z3rlimit 100"
+(* As defined in the NIST standard; pad, then update, then finish. *)
+let hash (a:hash_alg) (input:bytes{S.length input < max_input_length a}):
+  Tot (hash:lbytes (hash_length a))
+=
+  let padding = pad a (S.length input) in
+  finish a (update_multi a (init a) S.(input @| padding))
 
-let update_last (a:algorithm) prev len last chash = Spec.SHA2.update_last (alg a) prev len last chash
-
-let finish (a:algorithm) chash = Spec.SHA2.finish (alg a) chash
-
-let hash (a:algorithm) input = Spec.SHA2.hash (alg a) input
