specs/Spec.SHA1.fst
@@ -1,0 +1,255 @@
+module Spec.SHA1
+
+open Lib.IntTypes
+module H = Spec.Hash.Definitions
+module Seq = FStar.Seq
+
+open Spec.Hash.Definitions
+(* Source: https://nvlpubs.nist.gov/nistpubs/FIPS/NIST.FIPS.180-4.pdf *)
+
+(* Section 5.3.1 *)
+
+inline_for_extraction
+let init_as_list : list uint32 = [
+  u32 0x67452301;
+  u32 0xefcdab89;
+  u32 0x98badcfe;
+  u32 0x10325476;
+  u32 0xc3d2e1f0;
+]
+
+let h0 : words_state SHA1 = Seq.seq_of_list init_as_list
+
+let init = h0
+
+(* Section 6.1.2 Step 1: message schedule *)
+
+let rec w' (mi: Seq.lseq (word SHA1) block_word_length) (t: nat {t <= 79}) : GTot (word SHA1) (decreases (t)) =
+  if t < 16
+  then Seq.index mi (t)
+  else (w' mi (t - 3) ^. w' mi (t - 8) ^. w' mi (t - 14) ^. w' mi (t - 16)) <<<. 1ul
+
+let w (mi: Seq.lseq (word SHA1) block_word_length) (t: size_t {v t <= 79}) : GTot (word SHA1) = w' mi (v t)
+
+let compute_w_post
+  (mi: Seq.lseq (word SHA1) block_word_length)
+  (n: nat)
+  (res: Seq.lseq (word SHA1) n)
+: GTot Type0
+= (n <= 80 /\ (
+    forall (i: nat) . i < n ==> Seq.index res i == w' mi i
+  ))
+
+let compute_w_post_intro
+  (mi: Seq.lseq (word SHA1) block_word_length)
+  (n: nat)
+  (res: Seq.lseq (word SHA1) n)
+  (u: squash (n <= 80))
+  (f: (i: nat) -> Lemma
+      (requires (i < n))
+      (ensures (i < n /\ Seq.index res i == w' mi i)))
+: Lemma
+  (compute_w_post mi n res)
+= Classical.forall_intro (Classical.move_requires f)
+
+inline_for_extraction
+noextract
+let compute_w_n'
+  (mi: Seq.lseq (word SHA1) block_word_length)
+  (n: nat { n <= 79 } )
+  (w: ((i: nat {i < n}) -> Tot (y: word SHA1 {y == w' mi i})))
+: Tot (y: word SHA1 {y == w' mi n})
+= let r =
+      if n < 16
+      then Seq.index mi n
+      else (w (n - 3) ^. w (n - 8) ^. w (n - 14) ^. w (n - 16)) <<<. 1ul
+  in
+  r
+
+inline_for_extraction
+noextract
+let compute_w_n
+  (mi: Seq.lseq (word SHA1) block_word_length)
+  (n: nat { n <= 79 } )
+  (accu: Seq.lseq (word SHA1) n)
+: Pure (word SHA1)
+  (requires (compute_w_post mi n accu))
+  (ensures (fun y -> n <= 79 /\ y == w' mi n))
+= [@inline_let]
+  let w (i: nat {i < n}) : Tot (y: word SHA1 {y == w' mi i}) = Seq.index accu i in
+  compute_w_n' mi n w
+
+inline_for_extraction
+noextract
+let compute_w_next
+  (mi: Seq.lseq (word SHA1) block_word_length)
+  (n: nat { n <= 79 } )
+  (accu: Seq.lseq (word SHA1) n)
+: Pure (Seq.lseq (word SHA1) (n + 1))
+  (requires (compute_w_post mi n accu))
+  (ensures (fun accu' -> compute_w_post mi (n + 1) accu'))
+= let wn = compute_w_n mi n accu in
+  let accu' = Seq.snoc accu wn in
+  assert (n + 1 <= 80);
+  let g
+    (i: nat)
+  : Lemma
+    (requires (i < n + 1))
+    (ensures (i < n + 1 /\ Seq.index accu' i == w' mi i))
+  = if i = n
+    then ()
+    else ()
+  in
+  compute_w_post_intro mi (n + 1) accu' () g;
+  accu'
+
+let rec compute_w
+  (mi: Seq.lseq (word SHA1) block_word_length)
+  (n: nat)
+  (accu: Seq.lseq (word SHA1) n)
+: Pure (Seq.lseq (word SHA1) 80)
+  (requires (compute_w_post mi n accu))
+  (ensures (fun res -> compute_w_post mi 80 res))
+  (decreases (80 - n))
+= assert (n <= 80); // this assert is necessary for Z3 to prove that n <= 79 in the else branch
+  if n = 80
+  then accu
+  else compute_w mi (n + 1) (compute_w_next mi n accu)
+
+(* Section 4.1.1: logical functions *)
+
+inline_for_extraction
+let f (t: size_t {v t <= 79}) (x y z: word SHA1) : Tot (word SHA1) =
+  if t <. 20ul
+  then
+    (x &. y) ^. (~. x &. z)
+  else if 39ul <. t && t <. 60ul
+  then
+    (x &. y) ^. (x &. z) ^. (y &. z)
+  else
+    x ^. y ^. z
+
+(* Section 4.2.1 *)
+
+inline_for_extraction
+let k (t: size_t { v t <= 79 } ) : Tot (word SHA1) =
+  if t <. 20ul
+  then u32 0x5a827999
+  else if t <. 40ul
+  then u32 0x6ed9eba1
+  else if t <. 60ul
+  then u32 0x8f1bbcdc
+  else u32 0xca62c1d6
+
+(* Section 6.1.2 Step 3 *)
+
+let word_block = Seq.lseq (word SHA1) block_word_length
+
+let step3_body'_aux
+  (mi: word_block)
+  (st: words_state SHA1)
+  (t: size_t {v t < 80})
+  (wt: word SHA1 { wt == w mi t } )
+: Tot (words_state SHA1)
+= let sta = Seq.index st 0 in
+  let stb = Seq.index st 1 in
+  let stc = Seq.index st 2 in
+  let std = Seq.index st 3 in
+  let ste = Seq.index st 4 in
+  let _T = (sta <<<. 5ul) +. f t stb stc std +. ste +. k t +. wt in
+  let e = std in
+  let d = stc in
+  let c = stb <<<. 30ul in
+  let b = sta in
+  let a = _T in
+  let l : list uint32 = [
+    a;
+    b;
+    c;
+    d;
+    e;
+  ] in
+  assert_norm (List.Tot.length l = 5);
+  Seq.seq_of_list l
+  
+[@"opaque_to_smt"]
+let step3_body' = step3_body'_aux
+
+#reset-options "--z3rlimit 50"
+[@unifier_hint_injective]
+inline_for_extraction
+let step3_body_w_t
+  (mi: word_block)
+: Tot Type
+= (t: nat { t < 80 }) -> Tot (wt: word SHA1 { wt == w' mi t } )
+
+let step3_body
+  (mi: word_block)
+  (w: step3_body_w_t mi)
+  (st: words_state SHA1)
+  (t: nat {t < 80})
+: Tot (words_state SHA1)
+= step3_body' mi st (size t) (w t)
+
+inline_for_extraction
+let index_compute_w
+  (mi: word_block)
+  (cwt: Seq.lseq (word SHA1) 80 { compute_w_post mi 80 cwt } )
+: Tot (step3_body_w_t mi)
+= fun (t: nat {t < 80}) -> (Seq.index cwt t <: (wt: word SHA1 { wt == w' mi t }))
+
+let step3_aux
+  (mi: word_block)
+  (h: words_state SHA1)
+: Tot (words_state SHA1)
+= let cwt = compute_w mi 0 Seq.empty in
+  Spec.Loops.repeat_range 0 80 (step3_body mi (index_compute_w mi cwt)) h
+
+[@"opaque_to_smt"]
+let step3 = step3_aux
+
+(* Section 6.1.2 Step 4 *)
+
+let step4_aux
+  (mi: word_block)
+  (h: words_state SHA1)
+: Tot (words_state SHA1) =
+  let st = step3 mi h in
+  let sta = Seq.index st 0 in
+  let stb = Seq.index st 1 in
+  let stc = Seq.index st 2 in
+  let std = Seq.index st 3 in
+  let ste = Seq.index st 4 in
+  Seq.seq_of_list [
+    sta +. Seq.index h 0;
+    stb +. Seq.index h 1;
+    stc +. Seq.index h 2;
+    std +. Seq.index h 3;
+    ste +. Seq.index h 4;
+  ]
+
+[@"opaque_to_smt"]
+let step4 = step4_aux
+
+(* Section 3.1 al. 2: words and bytes, big-endian *)
+
+let words_of_bytes_block
+  (l: bytes { Seq.length l == block_length SHA1 } )
+: Tot word_block
+= words_of_bytes SHA1 #(block_word_length) l
+
+(* Section 6.1.2: outer loop body *)
+
+let update_aux h l =
+  let mi = words_of_bytes_block l in
+  step4 mi h
+
+let update = update_aux
+
+(* Section 5.1.1: padding *)
+
+let pad = Spec.Hash.PadFinish.pad SHA1
+
+(* Section 6.1.2: no truncation needed *)
+
+let finish = Spec.Hash.PadFinish.finish SHA1
